removing predicates and lemmas not needed,formatting.

src/Collections/Arrays/BinarySearch.dfy
@@ -3,113 +3,18 @@
 include "../../StandardLibrary.dfy"
 include "../../UInt.dfy"
 
+/*******************************************************************************
+*  Copyright by the contributors to the Dafny Project
+*  SPDX-License-Identifier: MIT 
+*******************************************************************************/
 
-
-module BinarySearch{
+module BinarySearch {
   export
-    reveals Reflexive, AntiSymmetric, Connected, TotalOrdering
-    reveals LexicographicByteSeqBelow, LexicographicByteSeqBelowAux
-    provides AboutLexicographicByteSeqBelow
     provides StandardLibrary, UInt
 
   import StandardLibrary
   import opened UInt = StandardLibrary.UInt
   import opened Wrappers = StandardLibrary.Wrappers
-  
-
-predicate Reflexive<T(!new)>(R: (T, T) -> bool) {
-    forall x :: R(x, x)
-  }
-
-predicate AntiSymmetric<T(!new)>(R: (T, T) -> bool) {
-    forall x, y :: R(x, y) && R(y, x) ==> x == y
-  }
-
-predicate Connected<T(!new)>(R: (T, T) -> bool) {
-    forall x, y :: R(x, y) || R(y, x)
-  }
-
-predicate TotalOrdering<T(!new)>(R: (T, T) -> bool) {
-    && Reflexive(R)
-    && AntiSymmetric(R)
-    && StandardLibrary.Transitive(R)
-    && Connected(R)
-  }
-
-predicate method LexicographicByteSeqBelow(x: seq<uint8>, y: seq<uint8>) {
-    LexicographicByteSeqBelowAux(x, y, 0)
-  }
-
-  predicate method LexicographicByteSeqBelowAux(x: seq<uint8>, y: seq<uint8>, n: nat)
-    requires n <= |x| && n <= |y|
-    decreases |x| - n
-  {
-    || n == |x|
-    || (n != |y| && x[n] < y[n])
-    || (n != |y| && x[n] == y[n] && LexicographicByteSeqBelowAux(x, y, n + 1))
-  }
-
-  lemma AboutLexicographicByteSeqBelow()
-    ensures TotalOrdering(LexicographicByteSeqBelow)
-  {
-    assert Reflexive(LexicographicByteSeqBelow) by {
-      forall x, n | 0 <= n <= |x| {
-        AboutLexicographicByteSeqBelowAux_Reflexive(x, n);
-      }
-    }
-    assert AntiSymmetric(LexicographicByteSeqBelow) by {
-      forall x, y, n: nat |
-        n <= |x| && n <= |y| && x[..n] == y[..n] &&
-        LexicographicByteSeqBelowAux(x, y, n) && LexicographicByteSeqBelowAux(y, x, n)
-      {
-        AboutLexicographicByteSeqBelowAux_AntiSymmetric(x, y, n);
-      }
-    }
-    assert StandardLibrary.Transitive(LexicographicByteSeqBelow) by {
-      forall x, y, z, n: nat |
-        n <= |x| && n <= |y| && n <= |z| &&
-        LexicographicByteSeqBelowAux(x, y, n) && LexicographicByteSeqBelowAux(y, z, n)
-      {
-        AboutLexicographicByteSeqBelowAux_Transitive(x, y, z, n);
-      }
-    }
-    assert Connected(LexicographicByteSeqBelow) by {
-      forall x, y, n: nat | n <= |x| && n <= |y| {
-        AboutLexicographicByteSeqBelowAux_Connected(x, y, n);
-      }
-    }
-  }
-
-  lemma AboutLexicographicByteSeqBelowAux_Reflexive(x: seq<uint8>, n: nat)
-    requires n <= |x|
-    ensures LexicographicByteSeqBelowAux(x, x, n)
-    decreases |x| - n
-  {
-  }
-
-  lemma AboutLexicographicByteSeqBelowAux_AntiSymmetric(x: seq<uint8>, y: seq<uint8>, n: nat)
-    requires n <= |x| && n <= |y|
-    requires x[..n] == y[..n]
-    requires LexicographicByteSeqBelowAux(x, y, n) && LexicographicByteSeqBelowAux(y, x, n)
-    ensures x == y
-    decreases |x| - n
-  {
-  }
-
-  lemma AboutLexicographicByteSeqBelowAux_Transitive(x: seq<uint8>, y: seq<uint8>, z: seq<uint8>, n: nat)
-    requires n <= |x| && n <= |y| && n <= |z|
-    requires LexicographicByteSeqBelowAux(x, y, n) && LexicographicByteSeqBelowAux(y, z, n)
-    ensures LexicographicByteSeqBelowAux(x, z, n)
-    decreases |x| - n
-  {
-  }
-
-  lemma AboutLexicographicByteSeqBelowAux_Connected(x: seq<uint8>, y: seq<uint8>, n: nat)
-    requires n <= |x| && n <= |y|
-    ensures LexicographicByteSeqBelowAux(x, y, n) || LexicographicByteSeqBelowAux(y, x, n)
-    decreases |x| - n
-  {
-  }
 
 method BinarySearch<T>(a: array<T>, key: T, compare: (T, T) -> bool) returns (r:Option<nat>)
   requires forall i,j :: 0 <= i < j < a.Length ==> compare(a[i], a[j]) || a[i] == a[j]
